kernel/uint63_63.ml
@@ -27,8 +27,6 @@ let to_int2 i = (0,i)
 
 let of_int64 _i = assert false
 
-let to_int_saturate i = i
-
 let of_float = int_of_float
 
 external to_float : int -> (float [@unboxed])
@@ -102,6 +100,10 @@ let lt (x : int) (y : int) =
 
 let le (x : int) (y : int) =
   (x lxor 0x4000000000000000) <= (y lxor 0x4000000000000000)
+[@@ocaml.inline always]
+
+let to_int_min n m =
+  if lt n m then n else m
 [@@ocaml.inline always]
 
     (* division of two numbers by one *)
