test-suite/primitive/float/frexp.v
@@ -1,5 +1,3 @@
-(* TODO add tests for ldexp (particularly with overflow with 31 and 63 bits integers) *)
-
 Require Import ZArith Floats.
 
 Definition denorm := Eval compute in ldexp one (-1074)%Z.
